theories/ProgramSemantics.v
@@ -8,16 +8,58 @@ Module SmallStep (syntax : WordSyntax)
                  (ST : StateType syntax)
                  (semantics : WordSemantics syntax ST) 
                  (model : MachineModel).
-  Module MM := model syntax.
-  Export syntax ST semantics MM.
+Module MM := model syntax.
+Export syntax ST semantics MM.
 
-  Definition nilprog : program := [].
-  Inductive pmstep : state -> program -> state -> Prop :=
-  | PMStepRefl : forall s,
-      pmstep s nilprog s
-  | PMStepMulti : forall wrd p p' s1 s2 s3,
-      step s1 wrd (Ok (s2, p')) ->
-      mem_well_typed s2.(mem) ->
-      pmstep s2 (p' ++ p) s3 ->
-      pmstep s1 (wrd :: p) s3.
+Definition nilprog : program := [].
+Inductive pmstep : state -> program -> state -> Prop :=
+| PMStepRefl : forall s,
+    pmstep s nilprog s
+| PMStepMulti : forall wrd p p' s1 s2 s3,
+    step s1 wrd (Ok (s2, p')) ->
+    mem_well_typed s2.(mem) ->
+    pmstep s2 (p' ++ p) s3 ->
+    pmstep s1 (wrd :: p) s3.
+
+Theorem pmstep_app_forward : forall p1 p2 s1 s2 s3,
+  pmstep s1 p1 s2 ->
+  pmstep s2 p2 s3 ->
+  pmstep s1 (p1 ++ p2) s3.
+Proof.
+  intros. revert s3 p2 H0.
+  induction H; intros; subst; simpl in *.
+    assumption.
+  econstructor. eassumption. assumption.
+  rewrite app_assoc. apply IHpmstep. assumption.
+Qed.
+
+Lemma pmstep_app_backward_gen :
+  forall s1 prog s3,
+    pmstep s1 prog s3 ->
+    forall p1 p2,
+      prog = p1 ++ p2 ->
+      exists s2, pmstep s1 p1 s2 /\ pmstep s2 p2 s3.
+Proof.
+  intros s1 prog s3 H. induction H; intros.
+    symmetry in H; apply app_eq_nil in H; destruct H; subst.
+    eexists. split; constructor.
+  destruct p1.
+    exists s1. split. constructor. simpl in H2; subst. econstructor.
+    eassumption. assumption. apply H1.
+  simpl in H2; inversion H2; subst; clear H2.
+  specialize (IHpmstep (p' ++ p1) p2).
+  rewrite app_assoc in IHpmstep. specialize (IHpmstep eq_refl).
+  destruct IHpmstep as (s4 & IHp1 & IHp2).
+  eexists. split. econstructor. eassumption. assumption.
+  eassumption. assumption.
+Qed.
+
+Lemma pmstep_app_backward : forall p1 p2 s1 s3,
+  pmstep s1 (p1 ++ p2) s3 ->
+  exists s2, pmstep s1 p1 s2 /\ pmstep s2 p2 s3.
+Proof.
+  intros.
+  apply (pmstep_app_backward_gen s1 (p1 ++ p2) s3 H p1 p2 eq_refl).
+Qed.
+
 End SmallStep.
