theories/ProofRules/Hoare.v
@@ -1,0 +1,160 @@
+From Stdlib Require Import NArith List.
+
+From Forq Require Import Syntax State ProgramSemantics MachineModel.
+From Forq.Words Require Import Word.
+
+Module Hoare (syntax : WordSyntax) 
+             (ST : StateType syntax) 
+             (semantics : WordSemantics syntax ST) 
+             (model : MachineModel).
+
+Module PS := SmallStep syntax ST semantics model.
+Import PS.
+
+Definition Assertion : Type := state -> Prop.
+
+Definition assert_implies (P Q : Assertion) : Prop :=
+  forall st, P st -> Q st.
+
+Declare Scope hoare_spec_scope.
+Open Scope hoare_spec_scope.
+
+Notation "P ->> Q" := (assert_implies P Q)
+                      (at level 80) : hoare_spec_scope.
+Notation "P <<->> Q" := (P ->> Q /\ Q ->> P)
+                          (at level 80) : hoare_spec_scope.
+
+Definition assert_of_Prop (P : Prop) : Assertion := fun _ => P.
+Coercion assert_of_Prop : Sortclass >-> Assertion.
+Add Printing Coercion assert_of_Prop.
+Arguments assert_of_Prop /.
+Add Printing Coercion assert_of_Prop.
+
+Declare Scope assertion_scope.
+Bind Scope assertion_scope with Assertion.
+Delimit Scope assertion_scope with assertion.
+
+Notation assert P := (P%assertion : Assertion).
+
+Notation "~ P" := (fun st => ~ assert P st) : assertion_scope.
+Notation "P /\ Q" := (fun st => assert P st /\ assert Q st) : assertion_scope.
+Notation "P \/ Q" := (fun st => assert P st \/ assert Q st) : assertion_scope.
+Notation "P -> Q" := (fun st => assert P st ->  assert Q st) : assertion_scope.
+Notation "P <-> Q" := (fun st => assert P st <->  assert Q st) : assertion_scope.
+
+Definition AssertionN : Type := state -> N.
+Definition AssertionN_of_N (n : N) : AssertionN :=
+  fun _ => n.
+Coercion AssertionN_of_N : N >-> AssertionN.
+Notation mkAssertN a := (a%assertion : AssertionN).
+
+Definition AssertionMem : Type := state -> memT.
+Definition AssertionMem_of_memT (m : memT) : AssertionMem :=
+  fun _ => m.
+Coercion AssertionMem_of_memT : memT >-> AssertionMem.
+Notation mkAssertMem m := (m%assertion : AssertionMem).
+
+Definition AssertionStack : Type := state -> stackT.
+Definition AssertionStack_of_stackT (l : stackT) : AssertionStack :=
+  fun _ => l.
+Coercion AssertionStack_of_stackT : stackT >-> AssertionStack.
+Notation mkAssertStack l := (l%assertion : AssertionStack).
+
+Definition AssertionDict : Type := state -> dictT.
+Definition AssertionDict_of_dictT (d : dictT) : AssertionDict :=
+  fun _ => d.
+Notation mkAssertDict d := (d%assertion : AssertionDict).
+
+(* Memory access *)
+Notation "@@ a" := (fun st => st.(mem) a) (at level 50) : assertion_scope.
+(* Stack access *)
+Notation "'.S'" := (fun st => st.(stack)) (at level 65) : assertion_scope.
+(* Dictionary access *)
+Notation "'WORDS' w" := (fun st => st.(dict) w) (at level 65) : assertion_scope.
+
+(* Notations for N (mostly for reasoning about memory) *)
+Notation "a = b" := (fun st => mkAssertN a st = mkAssertN b st) : assertion_scope.
+Notation "a <> b" := (fun st => mkAssertN a st <> mkAssertN b st) : assertion_scope.
+Notation "a <= b" := (fun st => mkAssertN a st <= mkAssertN b st) : assertion_scope.
+Notation "a < b" := (fun st => mkAssertN a st < mkAssertN b st) : assertion_scope.
+Notation "a >= b" := (fun st => mkAssertN a st >= mkAssertN b st) : assertion_scope.
+Notation "a > b" := (fun st => mkAssertN a st > mkAssertN b st) : assertion_scope.
+Notation "a + b" := (fun st => mkAssertN a st + mkAssertN b st) : assertion_scope.
+Notation "a - b" := (fun st => mkAssertN a st - mkAssertN b st) : assertion_scope.
+Notation "a * b" := (fun st => mkAssertN a st * mkAssertN b st) : assertion_scope.
+
+(* Notations for lists (mostly for reasoning about stack) *)
+Notation "a [=] b" := (fun st => mkAssertStack a st = mkAssertStack b st)
+  (at level 70, no associativity) : assertion_scope.
+Notation "a [<>] b" := (fun st => mkAssertStack a st <> mkAssertStack b st)
+  (at level 70, no associativity) : assertion_scope.
+Notation "a [::] b" := (fun st => a :: (mkAssertStack b st))
+  (at level 50, left associativity) : assertion_scope.
+Notation "a [++] b" := (fun st => (mkAssertStack a st) ++ (mkAssertStack b st))
+  (at level 50, left associativity) : assertion_scope.
+
+Definition valid_hoare_triple
+           (P : Assertion) (p : program) (Q : Assertion) : Prop :=
+  forall st st',
+     pmstep st p st' ->
+     P st  ->
+     Q st'.
+
+Notation "{{ P }} c {{ Q }}" :=
+  (valid_hoare_triple P c Q)
+    (at level 90)
+    : hoare_spec_scope.
+
+Theorem hoare_app : forall P Q R t1 t2,
+  {{P}} t1 {{Q}} ->
+  {{Q}} t2 {{R}} ->
+  {{P}} t1 ++ t2 {{R}}.
+Proof.
+  intros. unfold valid_hoare_triple in *. intros.
+  eapply pmstep_app_backward in H1.
+  destruct H1 as (s2 & Stept1 & Stept2).
+  eapply H0.
+    eassumption.
+  eapply H.
+    eassumption.
+  assumption.
+Qed.
+
+Theorem hoare_post_true : forall (P Q : Assertion) c,
+  (forall st, Q st) ->
+  {{P}} c {{Q}}.
+Proof.
+  intros. intros st st' _ _. apply H. 
+Qed.
+
+Theorem hoare_pre_false : forall (P Q : Assertion) c,
+  (forall st, ~ (P st)) ->
+  {{P}} c {{Q}}.
+Proof.
+  intros. intros st st' _ contra. exfalso. now apply (H st).
+Qed.
+
+Definition assertion_sub_stack (stack' : stackT) (P:Assertion) : Assertion :=
+  fun (st : state) =>
+    P {| stack := stack'; mem := st.(mem); dict := st.(dict) |}.
+Notation "P '[.S' := st ]" := (assertion_sub_stack st P)
+  (at level 10) : hoare_spec_scope.
+Definition assertion_push_stack (val : AssertionN) (P : Assertion) : Assertion :=
+  fun (st : state) =>
+    P {| stack := (val st) :: st.(stack); mem := st.(mem); dict := st.(dict) |}.
+Notation "P '[.S' :: v ]" := (assertion_push_stack (mkAssertN v) P)
+  (at level 10) : hoare_spec_scope.
+
+Definition assertion_sub_mem (a : addr) (v : N) (P:Assertion) : Assertion :=
+  fun (st : state) =>
+    P {| stack := st.(stack); mem := update st.(mem) a v; dict := st.(dict) |}.
+Notation "P '[@' a := v ]" := (assertion_sub_mem a v P)
+  (at level 10) : hoare_spec_scope.
+
+Definition assertion_sub_dict (a : addr) (p : program) (P:Assertion) : Assertion :=
+  fun (st : state) =>
+    P {| stack := st.(stack); mem := st.(mem); dict := update st.(dict) a p |}.
+Notation "P '[WORDS' a := p ]" := (assertion_sub_dict a p P)
+  (at level 10) : hoare_spec_scope.
+
+End Hoare.
