theories/ProofRules/Words/Core.v
@@ -1,0 +1,54 @@
+From Stdlib Require Import NArith.
+From Stdlib Require Import List.
+Import ListNotations.
+
+From Forq.ProofRules Require Import Hoare.
+From Forq.Words Require Import Word Core.
+From Forq Require Import Syntax State MachineModel.
+
+Module CoreHoare (ST : StateType CoreSyntax) 
+                 (model : MachineModel).
+Module SMX := CoreSemantics ST.
+Module H := Hoare CoreSyntax ST SMX model.
+Export H.
+Import ST.
+Open Scope hoare_spec_scope.
+
+Theorem hoare_literal : forall P (n : N),
+  {{ P[.S :: n] }} [Literal n] {{ P }}.
+Proof.
+  intros. unfold valid_hoare_triple. intros.
+  inversion H; clear H; subst. rewrite app_nil_r in H7.
+  inversion H3; clear H3; subst. inversion H7; clear H7; subst.
+  apply H0.
+Qed.
+
+Goal forall (s : stackT), {{ .S [=] s }} [Literal 5] {{ .S [=] (5 :: s : stackT) }}.
+  unfold valid_hoare_triple. intros.
+  inversion H; subst; clear H. inversion H3; subst; clear H3.
+  inversion H7; subst; clear H7. simpl. rewrite H0.
+  reflexivity.
+Qed.
+
+Goal forall addr tl, {{ .S [=] (addr :: tl : stackT) }} [Fetch] {{fun st => st.(stack) = st.(mem) addr :: tl }}.
+  unfold valid_hoare_triple. intros.
+  inversion H; subst; clear H. destruct st.
+  inversion H3; subst; clear H3.
+  inversion H7; subst; clear H7. simpl in *.
+  replace (mkAssertStack (addr :: tl : stackT) _) with (addr :: tl) in H0 by reflexivity.
+  inversion H0; subst; clear H0. reflexivity.
+Qed.
+
+Theorem hoare_fetch : forall P (addr : N),
+  {{ P[.S :: @@ addr] }} [Fetch] {{ P[.S :: addr] }}.
+Proof.
+  unfold valid_hoare_triple, assertion_push_stack. intros.
+  destruct st, st'. simpl in *.
+  replace ((mkAssertN addr) _) with addr by reflexivity.
+  destruct stack0. inversion H; inversion H3.
+  inversion H; subst; clear H. rewrite app_nil_r in H7.
+  inversion H3; subst; clear H3; simpl in *.
+  inversion H7; subst; clear H7.
+Abort.
+
+End CoreHoare.
